\documentclass[addpoints]{exam}
\usepackage{amsmath}
\usepackage{amsfonts}
\usepackage[most]{tcolorbox}
\usepackage{tikz}
\usepackage{pgfplots}
\usepackage{mdframed}
\usepackage{hyperref}
\usepackage{amsthm}

\marksnotpoints
\pointsinrightmargin
\bracketedpoints
\printanswers

\hypersetup{
  colorlinks=true,
  linkcolor=blue,
  filecolor=magenta,
  urlcolor=blue,
  pdfpagemode=FullScreen,
}

\urlstyle{same}

\pagestyle{headandfoot}
\firstpageheadrule
\runningheadrule
\firstpageheader{Pre Calc Prep}{Trig PSET}{Shah}
\runningheader{}{Trig}{}
\firstpagefooter{}{}{}
\runningfooter{ }{\thepage}{ }

\begin{document}
  \vspace{1in}

  \noindent\makebox[\textwidth]{Name:\enspace\hrulefill}

  \vspace{.1in}

  \begin{center}
      \fbox{\fbox{\parbox{5.5in}{\centering
      Answer the questions in the spaces provided on the following pages.  If you run out of room for an answer, continue on the back of the page. Show \textbf{all} your work!}}}
  \end{center}
  
  \begin{questions}
    \question Write a recursive and generic formula for the following sequences
    \begin{parts}
      \part $a_n = \{1, 2, 3, 4, \ldots, n\}$
      \begin{solution}[\stretch{1}]
        \begin{minipage}{0.45\linewidth}
          \begin{center}
            \underline{Generic}
          \end{center}
          \[
            a_n = n
          \]
        \end{minipage}
        \hfill 
        \begin{minipage}{0.45\linewidth}
          \begin{center}
            \underline{Recursive}
          \end{center}
          \[
            a_{n+1} = n + 1 \text{;} \hspace{0.1in} a_1 = 1
          \]
        \end{minipage}
      \end{solution}

      \part $a_n = \{3, 6, 9, 12, \ldots, n\}$
      \begin{solution}[\stretch{1}]
        \begin{minipage}{0.45\linewidth}
          \begin{center}
            \underline{Generic}
          \end{center}
          \[
            a_n = 3 + 3(n-1) = 3n
          \]
        \end{minipage}
        \hfill 
        \begin{minipage}{0.45\linewidth}
          \begin{center}
            \underline{Recursive}
          \end{center}
          \[
            a_{n+1} = 3 + a_{n} \text{;} \hspace{0.1in} a_1 = 3
          \]
        \end{minipage}
      \end{solution}

      \part $a_n = \{1, 3, 9, 27, \ldots, n\}$ 
      \begin{solution}[\stretch{1}]
        \begin{minipage}{0.45\linewidth}
          \begin{center}
            \underline{Generic}
          \end{center}
          \[
            a_n = 3^n
          \]
        \end{minipage}
        \hfill 
        \begin{minipage}{0.45\linewidth}
          \begin{center}
            \underline{Recursive}
          \end{center}
          \[
            a_{n+1} = 3\left(a_n\right) \text{;} \hspace{0.1in} a_1 = 1
          \]
        \end{minipage}
      \end{solution}

      \part $\displaystyle\,a_n = \{\frac{1}{2}, \frac{1}{4}, \frac{1}{8}, \ldots, n\}$ 
      \begin{solution}[\stretch{1}]
        \begin{minipage}{0.45\linewidth}
          \begin{center}
            \underline{Generic}
          \end{center}
          \vspace{0.1in}
          \[
            a_n = \left(\frac{1}{2}\right)^n
          \]
        \end{minipage}
        \hfill 
        \begin{minipage}{0.45\linewidth}
          \begin{center}
            \underline{Recursive}
          \end{center}
          \vspace{0.1in}
          \[
            a_{n+1} = \frac{1}{2}\left(a_n\right) \text{;} \hspace{0.1in} a_1 = \frac{1}{2}
          \]
        \end{minipage}
      \end{solution}
    \end{parts}

    \question Rewrite the series $\displaystyle\, \sum\limits_{n=0}^{12} \frac{n+2}{3}$ to start at $n=3$
    \begin{solution}[\stretch{1}]
      \[
        \sum\limits_{n=3}^{15} \frac{n-3+2}{3} = \sum\limits_{n=3}^{15} \frac{n-1}{3}
      \]      
    \end{solution}

    \question Rewrite the series $\displaystyle\, \sum\limits_{n=5}^{20} \frac{n}{(n-1)^2}$ to start at $n=0$
    \begin{solution}[\stretch{1}]
      \[
        \sum\limits_{n=0}^{15} \frac{n+5}{(n+5-1)^2} = \sum\limits_{n=0}^{15} \frac{n+5}{(n-4)^2}
      \]
    \end{solution}

    \newpage 

    \question Strip out the last term of the sum $\displaystyle\, \sum\limits_{n=0}^{22} \frac{n+8}{3}$ 
    \begin{solution}[\stretch{1}]
      \[
        \frac{22+8}{3} + \sum\limits_{n=0}^{21} \frac{n+8}{3} = 10 + \sum\limits_{n=0}^{21} \frac{n+8}{3}
      \]
    \end{solution}

    \question Rewrite the following expression as a single summation, $\displaystyle\, \sum\limits_{i=0}^{k} i^3 + \left(k+1\right)^3$
    \begin{solution}[\stretch{1}]
      \[
        \sum\limits_{n=0}^{k+1} i^3 
      \]
    \end{solution}

    \question Write the following in summation notation $\displaystyle\, \frac{1}{2} + \frac{2}{3^2} + \frac{3}{4^3} + \cdots + \frac{n}{\left(n+1\right)^n}$ 
    \begin{solution}[\stretch{1}]
      \[
        \sum\limits_{k=1}^{n} \frac{k}{\left(k+1\right)^k}
      \]
    \end{solution}

    \question Write the following expression as a single summation: $\displaystyle\, 3 * \sum\limits_{t=1}^{p} \left(2t-3\right) + \sum\limits_{t=1}^{p} \left(4-5t\right)$
    \begin{solution}[\stretch{1}]
      \begin{align*}
        3 * \sum\limits_{t=1}^{p} \left(2t-3\right) + \sum\limits_{t=1}^{p} \left(4-5t\right) &= \sum\limits_{t=1}^{p} \left(6t-9\right) + \sum\limits_{t=1}^{p} \left(4-5t\right) \\ 
        &= \sum\limits_{t=1}^{p} t-5
      \end{align*}
    \end{solution}
  \end{questions}
\end{document}
