\documentclass[addpoints]{exam}
\usepackage{amsmath}
\usepackage{amsfonts}
\usepackage[most]{tcolorbox}
\usepackage{tikz}
\usepackage{pgfplots}
\usepackage{mdframed}
\usepackage{hyperref}
\usepackage{amsthm}

\marksnotpoints
\pointsinrightmargin
\bracketedpoints
\printanswers

\hypersetup{
  colorlinks=true,
  linkcolor=blue,
  filecolor=magenta,
  urlcolor=blue,
  pdfpagemode=FullScreen,
}

\urlstyle{same}

\pagestyle{headandfoot}
\firstpageheadrule
\runningheadrule
\firstpageheader{Pre Calc Prep}{Trig PSET}{Shah}
\runningheader{}{Trig}{}
\firstpagefooter{}{}{}
\runningfooter{ }{\thepage}{ }

\begin{document}
  \vspace{1in}

  \noindent\makebox[\textwidth]{Name:\enspace\hrulefill}

  \vspace{.1in}

  \begin{center}
      \fbox{\fbox{\parbox{5.5in}{\centering
      Answer the questions in the spaces provided on the following pages.  If you run out of room for an answer, continue on the back of the page. Show \textbf{all} your work!}}}
  \end{center}

  \begin{questions}
    \question Prove the following identity: $\displaystyle\, \frac{\sec^2 x}{\sec^2 x - 1} = \csc^2 x$ 
    \begin{solution}[\stretch{1}]
      \begin{align*}
         \csc^2 x &= \frac{\sec^2 x}{\sec^2 x - 1} \\ 
         &= \frac{\sec^2 x}{\tan^2 x} \\ 
         &= \sec^2 x \cot^2 x \\ 
         &= \frac{1}{\cos^2 x} \frac{\cos^2 x}{\sin^2 x} \\ 
         &= \frac{1}{\sin^2 x} \\ 
         &= \csc^2 x
      \end{align*}
    \end{solution}

    \question Prove the following identity: $\displaystyle\, \csc^2 x \tan^2 x - 1 = \tan^2 x$
    \begin{solution}[\stretch{1}]
      \begin{align*}
        \tan^2 x &= \csc^2 x \tan^2 x - 1 \\ 
        &= \frac{1}{\sin^2 x}\frac{\sin^2 x}{\cos^2 x} - 1 \\ 
        &= \frac{1}{\cos^2 x} - 1 \\ 
        &= \sec^2 x - 1 \\ 
        &= \tan^2 x
      \end{align*}
    \end{solution}

    \newpage

    \question Prove the following identity: $\displaystyle\, \tan^2 x \sin^2 x = \tan^2 x - \sin^2 x$ 
    \begin{solution}[\stretch{1}]
      \begin{align*}
        \tan^2 x \sin^2 x &= \tan^2 x - \sin^2 x \\ 
        &= \tan^2 x - \sin^2 x \left(\frac{\cos^2 x}{\cos^2 x}\right) \\ 
        &= \tan^2 x - \frac{\left(\sin^2 x\right)\left(\cos^2 x\right)}{\cos^2 x} \\ 
        &= \tan^2 x - \frac{\sin^2 x}{\cos^2 x}\left(\cos^2 x\right) \\ 
        &= \tan^2 x - \tan^2 x \cos^2 x \\ 
        &= \tan^2 x \left(1 - \cos^2 x\right) \\ 
        &= \tan^2 x \sin^2 x
      \end{align*}
    \end{solution}

    \question Prove the following identity: $\displaystyle\, \frac{\cos x + 1}{\sin^3 x} = \frac{\csc x}{1-\cos x}$ 
    \begin{solution}[\stretch{1}]
      \begin{align*}
        \frac{\cos x + 1}{\sin^3 x} &= \frac{\csc x}{1 - \cos x} \\
        &= \frac{1}{\sin x}\frac{\cos x + 1}{\sin ^2 x} \\ 
        &= \left(\csc x\right)\frac{\cos x + 1}{1 - \cos^2 x} \\ 
        &= \left(\csc x\right)\frac{\cos x + 1}{\left(1 - \cos x\right)\left(1 + \cos x\right)} \\ 
        &= \left(\csc x\right)\frac{1}{1 - \cos x} \\ 
        &= \frac{\csc x}{1 - \cos x}
      \end{align*}
    \end{solution}

    \newpage

    \question \textbf{Bonus \underline{extra hard} question:} Prove the following identity: $\displaystyle\, \frac{1 + \tan^2 x}{\sec x} = \sqrt{\frac{1}{\frac{1}{2}\left(1 - \cos(2x)\right)}}$ 
    \begin{solution}[\stretch{1}]
      \begin{align*}
        \frac{1 + \tan^2 x}{\sec x} &= \sqrt{\frac{1}{\frac{1}{2}\left(1 - \cos(2x)\right)}} \\ 
        \frac{1 + \tan^2 x}{\sec x} &= \sqrt{\frac{1}{2 - 1 - \cos(2x)}} \\ 
        \frac{1 + \tan^2 x}{\sec x} &= \sqrt{\frac{1}{\frac{1}{2}\left(2 - 1 - \cos(2x)\right)}} \\ 
        \frac{1 + \tan^2 x}{\sec x} &= \sqrt{\frac{1}{1 - \frac{1 - \cos(2x)}{2}}} \\ 
        \frac{1 + \tan^2 x}{\sec x} &= \sqrt{\frac{1}{1 - \sin^2 x}} \\ 
        \frac{1 + \tan^2 x}{\sec x} &= \sqrt{\frac{1}{\cos^2 x}} \\ 
        \frac{1 + \tan^2 x}{\sec x} &= \sqrt{\sec^2 x} \\ 
        \frac{\sec^2 x}{\sec x} &= \sec x \\ 
        \sec x &= \sec x
      \end{align*}
    \end{solution}
  \end{questions}
\end{document}
